VSUpile now entirely works in current VSU system

progs/VSUpile/fast/verif_fastcore.v
@@ -1,8 +1,6 @@
 Require Import VST.floyd.proofauto.
 Require Import VST.floyd.VSU.
 
-Require Import VST.floyd.linking.
-
 Require Import spec_stdlib.
 
 Require Import verif_stdlib.
@@ -11,131 +9,22 @@ Require Import verif_fastonepile.
 Require Import verif_fastapile.
 Require Import verif_fasttriang.
 
-Section CORE_VSU.
-Variable M: MallocFreeAPD.
-Definition PrivPILE: spec_fastpile_private.FastpilePrivateAPD:= PILEPRIV M.
+Definition PrivPILE: spec_fastpile_private.FastpilePrivateAPD := PILEPRIV M.
 Definition PILE: spec_fastpile.PileAPD := spec_fastpile_private.pilepreds PrivPILE. 
 
 Definition ONEPILE : spec_onepile.OnePileAPD := ONEPILE PILE.
 
-Definition onepile_pile_prog: Clight.program := 
-  match link_progs fastpile.prog onepile.prog with
-    Errors.OK p => p
-  | _ => fastpile.prog (*arbitrary*)
-  end.
-Definition mrg_prog1 := ltac:
-  (let x := eval hnf in onepile_pile_prog in
-   let x := eval simpl in x in 
-   let x := eval compute in x in 
-       exact x).
-Instance mrg_cs1 : compspecs. make_compspecs mrg_prog1. Defined.
+Definition Onepile_Pile_VSU :=
+  ltac:(linkVSUs (PilePrivateVSU M) (OnepileVSU M PILE) ). 
 
-Definition mrg_Vprog1:varspecs. mk_varspecs mrg_prog1. Defined.
+Definition Apile_Onepile_Pile_VSU :=
+  ltac:(linkVSUs (Onepile_Pile_VSU) (ApileVSU M PrivPILE)). 
 
-Definition mrg_Imports1:funspecs := (MF_ASI M).
+Definition Triang_Apile_Onepile_Pile_VSU :=
+  ltac:(linkVSUs Apile_Onepile_Pile_VSU (TriangVSU M PILE)). 
 
-Definition mrg_Exports1:funspecs := 
-G_merge (spec_fastpile.PileASI M PILE) (spec_onepile.OnepileASI M ONEPILE).
-
-Definition Onepile_Pile_VSU:
-@VSU NullExtension.Espec
-   mrg_Vprog1 mrg_cs1 nil mrg_Imports1 mrg_prog1 mrg_Exports1 (one_pile PILE None).
-Proof.
-  VSULink_tac (PilePrivateVSU M) (OnepileVSU M PILE).
-  extensionality gv. simpl. rewrite emp_sepcon; trivial.
-Qed.
-
-Definition APILE := verif_fastapile.APILE (*M*) PrivPILE.
-
-Definition apile_onepile_pile_prog: Clight.program := 
-  match link_progs mrg_prog1 fastapile.prog with
-    Errors.OK p => p
-  | _ => apile.prog (*arbitrary*)
-  end.
-Definition mrg_prog2 := ltac:
-  (let x := eval hnf in apile_onepile_pile_prog in
-   let x := eval simpl in x in 
-   let x := eval compute in x in 
-       exact x).
-
-Instance mrg_cs2 : compspecs. make_compspecs mrg_prog2. Defined.
-
-Definition mrg_Vprog2:varspecs. mk_varspecs mrg_prog2. Defined.
-
-Definition mrg_Imports2:funspecs := MF_ASI M.
-
-Definition mrg_Exports2:funspecs := G_merge  mrg_Exports1 (Apile_ASI M PrivPILE).
-
-Definition Apile_Onepile_Pile_VSU:
-@VSU NullExtension.Espec
-   mrg_Vprog2 mrg_cs2 nil mrg_Imports2 mrg_prog2 mrg_Exports2
-   (fun gv => one_pile PILE None gv * apile PrivPILE [] gv)%logic.
-Proof.
-  VSULink_tac (Onepile_Pile_VSU) (ApileVSU M PrivPILE).
-  extensionality gv; trivial.
-Qed.
-
-Definition triang_apile_onepile_pile_prog: Clight.program := 
-  match link_progs mrg_prog2 triang.prog with
-    Errors.OK p => p
-  | _ => triang.prog (*arbitrary*)
-  end.
-Definition mrg_prog3 := ltac:
-  (let x := eval hnf in triang_apile_onepile_pile_prog in
-   let x := eval simpl in x in 
-   let x := eval compute in x in 
-       exact x).
-
-Instance mrg_cs3 : compspecs. make_compspecs mrg_prog3. Defined.
-
-Definition mrg_Vprog3:varspecs. mk_varspecs mrg_prog3. Defined.
-
-Definition mrg_Imports3:funspecs := MF_ASI M.
-
-Definition mrg_Exports3:funspecs := G_merge mrg_Exports2 (spec_triang.TriangASI M).
-
-Definition Triang_Apile_Onepile_Pile_VSU:
-@VSU NullExtension.Espec
-   mrg_Vprog3 mrg_cs3 nil mrg_Imports3 mrg_prog3 mrg_Exports3
-  (fun gv => one_pile PILE None gv * apile PrivPILE [] gv)%logic.
-Proof.
-  VSULink_tac (Apile_Onepile_Pile_VSU) (TriangVSU M PILE).
-  extensionality gv. normalize.
-Qed.
-
-Definition mm_triang_apile_onepile_pile_prog: Clight.program := 
-  match link_progs stdlib.prog mrg_prog3 with
-    Errors.OK p => p
-  | _ => triang.prog (*arbitrary*)
-  end.
-Definition coreprog := ltac:
-  (let x := eval hnf in mm_triang_apile_onepile_pile_prog in
-   let x := eval simpl in x in 
-   let x := eval compute in x in 
-       exact x).
-
-Instance coreCS : compspecs. make_compspecs coreprog. Defined.
-
-Definition coreVprog:varspecs. mk_varspecs coreprog. Defined.
-
-Definition coreImports:funspecs := nil.
-
-Definition coreExports:funspecs := G_merge (MF_ASI M) mrg_Exports3.
-
-Definition coreBuiltins:funspecs := (MallocFreeASI M). (*i.e. MF_E M*)
-
-Definition Core_VSU:
-@VSU NullExtension.Espec coreVprog coreCS coreBuiltins coreImports coreprog coreExports
-     (fun gv => one_pile PILE None gv * apile PrivPILE [] gv)%logic.
-Proof.
-  VSULink_tac (MallocFreeVSU M) (Triang_Apile_Onepile_Pile_VSU).
-  extensionality gv. normalize.
-Qed.
-
-Definition Core_CanVSU: @CanonicalVSU NullExtension.Espec
-   coreVprog coreCS coreBuiltins coreImports coreprog coreExports
-   (fun gv => one_pile PILE None gv * apile PrivPILE [] gv)%logic.
-Proof.
-eapply VSU_to_CanonicalVSU. apply Core_VSU.
-Qed.
-End CORE_VSU.
+Definition Core_VSU :=
+  privatizeExports 
+  ltac:(linkVSUs MallocFreeVSU Triang_Apile_Onepile_Pile_VSU)
+  [stdlib._malloc; stdlib._free; stdlib._exit; fastpile._Pile_new;
+   fastpile._Pile_add; fastpile._Pile_count; fastpile._Pile_free].
