progs/VSUpile/simple_verif_linked_main.v
@@ -10,61 +10,38 @@ Require Import simple_spec_apile.
 Require Import simple_spec_triang.
 Require Import main.
 Require Import simple_spec_main.
+Require Import simple_verif_stdlib.
+Require Import simple_verif_pile.
+Require Import simple_verif_onepile.
+Require Import simple_verif_apile.
+Require Import simple_verif_triang.
 
-Section MainInstASI.
-  Variable G: list (globals -> mpred).
+Definition Onepile_Pile_VSU :=
+  ltac:(linkVSUs PileVSU OnepileVSU). 
 
-(*Specification of "module-instantiated main" - we permit an arbitrary G here
- (eventually, we'll roll M (or better: memmrg M gv) into G, too.*)
-Definition main_inst_spec:=
- DECLARE _main
- WITH gv: globals
- PRE [ ] 
-    PROP ()
-    PARAMS () GLOBALS (gv)
-    SEP (fold_right (fun g p => g gv * p) emp G; has_ext tt)
- POST[ tint ]
-    PROP()
-    LOCAL(temp ret_temp (Vint (Int.repr 0)))
-    SEP(mem_mgr gv; has_ext tt; TT).
-End MainInstASI.
+Definition Apile_Onepile_Pile_VSU :=
+  ltac:(linkVSUs Onepile_Pile_VSU ApileVSU). 
 
-Definition linked_prog : Clight.program :=
- ltac: (linking.link_progs_list [
-   stdlib.prog; pile.prog; onepile.prog; apile.prog;
-   triang.prog; main.prog]).
+Definition Triang_Apile_Onepile_Pile_VSU :=
+  ltac:(linkVSUs Apile_Onepile_Pile_VSU TriangVSU). 
 
-Instance LinkedCompSpecs : compspecs. make_compspecs linked_prog. Defined.
+Definition Core_VSU :=
+  privatizeExports 
+  ltac:(linkVSUs MallocFreeVSU Triang_Apile_Onepile_Pile_VSU)
+  [stdlib._malloc; stdlib._free; stdlib._exit; pile._Pile_new;
+   pile._Pile_add; pile._Pile_count; pile._Pile_free].
 
-Definition LinkedVprog : varspecs. mk_varspecs linked_prog. Defined.
+Instance CompSpecs : compspecs. make_compspecs prog. Defined.
+Definition whole_prog := ltac:(QPlink_progs (QPprog prog) (VSU_prog Core_VSU)).
+Definition Vprog: varspecs := QPvarspecs whole_prog.
+Definition Main_imports := VSU_Exports Core_VSU. 
+Definition mainspec :=  main_spec whole_prog.
+Definition Gprog := mainspec :: Main_imports.
 
-(*Instantiating main_spec with linked_prog rather than main.prog ensures that all 
-  gv's are present after we do start_function in body_main*)
-Definition mainspec (*M*) := (main_spec (*M*) linked_prog).
-
-  Definition MainImports: funspecs := OnepileASI ++ ApileASI ++ TriangASI.
-
-  Definition MyInitPred := [(*mem_mgr M; *)onepile None; apile nil].
-  Definition maininstspec (*M*) := (main_inst_spec MyInitPred).
-  
-  Definition main_internal_specs: funspecs := [main_spec linked_prog].
-
-  Definition MainVprog : varspecs. mk_varspecs main.prog. Defined.
-
-  Definition MainGprog:funspecs := MainImports ++ main_internal_specs.
-
-  (* Instance MainCompSpecs : compspecs. make_compspecs main.prog. Defined.
-     Definition MainVprog : varspecs. mk_varspecs main.prog. Defined.*)
-
- (* Again, to ensure that start_function succeeds, we use LinkedCompSpecs and
-    LinkedVprog*)
-  Lemma body_main: semax_body LinkedVprog MainGprog f_main maininstspec.
+Lemma body_main: semax_body Vprog Gprog f_main mainspec.
 Proof.
+pose Core_VSU.
 start_function.
-sep_apply (make_mem_mgr gv).
-unfold MyInitPred, fold_right.
-Intros.
-
 forward_call gv.
 forward_for_simple_bound 10
   (EX i:Z,
@@ -88,160 +65,19 @@ compute; split; congruence.
 forward_call (10,gv).
 lia.
 forward.
-cancel.
 Qed.
 
-Require Import simple_verif_core.
-Require Import VST.veric.initial_world.
-
-(*Finally, we assert existence of a mallocfree library.*)
-
-Lemma tc_VG: tycontext_subVG LinkedVprog MainGprog
-                             LinkedVprog (mainspec :: coreExports).
-Proof. split.
-* intros i. red. rewrite 2 semax_prog.make_context_g_char, 2 make_tycontext_s_find_id by LNR_tac.
-  remember (find_id i MainGprog) as w.
-  destruct w; [symmetry in Heqw | simpl; trivial].
-  +  simpl in Heqw.
-     repeat (if_tac in Heqw; [ subst i; inv Heqw; reflexivity |]).
-     congruence.
-  + repeat (if_tac; [subst i; simpl; trivial |]); trivial.
-* intros i; red. rewrite 2 make_tycontext_s_find_id.
-  remember (find_id i MainGprog) as w.
-  destruct w; [symmetry in Heqw | trivial]. simpl in Heqw.
-  repeat (if_tac in Heqw; [ subst i; inv Heqw;
-                            eexists; split; [ reflexivity | apply funspec_sub_si_refl]
-                          | ]).
-  congruence.
-Qed.
-
-Definition ExtIDtable : PTree.t unit :=
-  ltac:(let x := constr:(fold_right (fun i t => PTree.set i tt t) (PTree.empty _) (ExtIDs linked_prog))
-           in let x := eval compute in x
-           in exact x).
-
-Definition in_ExtIDs (ia: ident*funspec) : bool :=
- match PTree.get (fst ia) ExtIDtable with Some _ => true | None => false end.
-
-Definition LinkedSYS_pre:funspecs :=
-   filter in_ExtIDs (augment_funspecs linked_prog MallocFreeASI).
-
-Definition LinkedSYS:funspecs := 
-  ltac: 
-    (let x := eval hnf in LinkedSYS_pre in
-     let x := eval simpl in x in 
-     (*let x := eval compute in x in leaving this in leads Coq to timeout/crash*)
-       exact x).
-
-Lemma ApplibSys_in_LinkedSys: forall i phi, find_id i coreBuiltins = Some phi -> find_id i LinkedSYS = Some phi.
-  Proof.
-    intros. specialize (find_id_In_map_fst _ _ _ H); intros.
-    simpl in H0. repeat (destruct H0 as [HO | H0]; [ subst i; inv H; reflexivity |]). contradiction.
-  Qed. 
-
-Lemma LinkedSYS_External: forall i, In i (map fst LinkedSYS) ->
-      exists ef ts t cc, find_id i (prog_defs linked_prog) = Some (Gfun (External ef ts t cc)).
-  Proof.
-    intros. cbv in H. 
-    repeat (destruct H as [H | H];
-      [ subst; try solve [do 4 eexists; split; reflexivity ]
-      | ]).
-    contradiction.
-  Qed.
-
-Lemma LinkedSYS_vacuous i phi: find_id i LinkedSYS = Some phi -> find_id i coreBuiltins = None ->
-        exists ef argsig retsig cc, 
-           phi = vacuous_funspec (External ef argsig retsig cc) /\ 
-           find_id i (prog_funct coreprog) = Some (External ef argsig retsig cc) /\
-           ef_sig ef = {| sig_args := typlist_of_typelist argsig;
-                          sig_res := rettype_of_type retsig;
-                          sig_cc := cc_of_fundef (External ef argsig retsig cc) |}.
-  Proof.
-    intros. specialize (find_id_In_map_fst _ _ _ H); intros.
-    cbv in H1.
-    Time repeat (destruct H1 as [H1 | H1]; 
-      [ subst; inv H; try solve [do 4 eexists; split3; reflexivity]
-      | ]); try inv H0; try contradiction. (*3s*)
-  Qed.
-
-Lemma disjoint_Vprog_linkedfuncts: 
-      list_disjoint (map fst LinkedVprog) (map fst (prog_funct linked_prog)).
+Definition MainComp:  MainCompType nil (QPprog prog) Core_VSU whole_prog (snd (main_spec whole_prog))  emp.
 Proof.
-  intros x y X Y ?; subst x; cbv in X; apply assoclists.find_id_None_iff in Y; [ trivial | clear H Y];
-  repeat (destruct X as [X | X]; [ subst y; cbv; reflexivity |]); contradiction.
+mkComponent prog.
+solve_SF_internal body_main.
 Qed.
 
-Lemma main_sub: funspec_sub (snd (main_inst_spec MyInitPred))
-                             (snd mainspec).
-Proof. do_funspec_sub. unfold main_pre; simpl; Intros; subst. clear. 
-  Exists (initialize.genviron2globals g) emp. unfold globvars2pred; simpl.
-  unfold globvars2pred, lift2; Intros. simpl. entailer!.
-  + intros. entailer!.
-  + rewrite sepcon_comm; apply sepcon_derives.
-    - eapply derives_trans. 2: apply simple_verif_onepile.onepile_Init; auto.
-      unfold InitGPred. simpl. unfold globvar2pred; simpl. rewrite ! sepcon_emp.
-      apply andp_right.
-      * eapply derives_trans. apply mapsto_zeros_memory_block.
-        apply writable_readable. apply writable_Ews.
-        rewrite memory_block_isptr; Intros.
-        apply prop_right.
-        unfold initialize.genviron2globals in *.
-        destruct (Map.get g onepile._the_pile); try contradiction; auto.
-        eexists; reflexivity.       
-      * unfold globvar2pred. simpl; auto.
-    - unfold globvar2pred; simpl. rewrite mapsto_isptr; Intros.
-       assert (headptr (initialize.genviron2globals g apile._a_pile)).
-        unfold initialize.genviron2globals in *.
-        destruct (Map.get g apile._a_pile); try contradiction; auto.
-        eexists; reflexivity.    
-      eapply derives_trans; [ | apply simple_verif_apile.make_apile; trivial].
-      rewrite sepcon_emp.
-      erewrite <- (mapsto_data_at''); trivial. apply derives_refl.
-Qed.
+Lemma WholeComp: WholeCompType Core_VSU MainComp.
+Proof. proveWholeComponent. Qed.
 
-Definition Imports:funspecs:=nil.
-(*
-Lemma CSSUB: cspecs_sub MainCompSpecs LinkedCompSpecs.
-Proof.
-  split3.
-+ intros i; red; remember ((@cenv_cs MainCompSpecs) ! i) as w; destruct w; 
-   [symmetry in Heqw; simpl in Heqw; rewrite PTree.gleaf in Heqw; congruence | trivial].
-+ intros i. red. remember ((@ha_env_cs MainCompSpecs) ! i) as w. destruct w; [symmetry in Heqw | trivial].
-  simpl in Heqw. rewrite PTree.gleaf in Heqw. congruence.
-+ intros i. red. remember ((@la_env_cs MainCompSpecs) ! i) as w. destruct w; [symmetry in Heqw | trivial].
-  simpl in Heqw. rewrite PTree.gleaf in Heqw. congruence.
-Qed.*)
+Lemma WholeProgSafe: WholeProgSafeType WholeComp tt.
+Proof. proveWholeProgSafe. Qed.
 
-Require Import VST.floyd.VSU_addmain.
+Eval red in WholeProgSafeType WholeComp tt.
 
-Definition SO_VSU: @LinkedProgVSU NullExtension.Espec LinkedVprog LinkedCompSpecs
-      LinkedSYS Imports linked_prog [mainspec (*M*)]
-      (fun gv => onepile None gv * apile  [] gv)%logic.
-Proof.
- VSUAddMain_tac Core_CanVSU.
-   + apply disjoint_Vprog_linkedfuncts.
-   + apply LinkedSYS_External.
-   + eapply semax_body_subsumption.
-       * eapply semax_body_funspec_sub. 
-         - apply body_main.
-         - apply main_sub.
-         - LNR_tac.
-       * apply tycontext_sub_i99. apply tc_VG.
-   + apply LinkedSYS_vacuous.
-Qed.
-
-Lemma prog_correct:
-  exists G, 
- @semax_prog NullExtension.Espec LinkedCompSpecs linked_prog tt LinkedVprog G.
-Proof.
-  destruct SO_VSU as [G Comp MAIN]. exists G. 
-  assert (DomG: map fst G = map fst (prog_funct linked_prog)).
-  { destruct Comp. unfold Comp_G in *. rewrite CC_canonical.
-    cbv; reflexivity. }
-  prove_linked_semax_prog.
-  all: rewrite augment_funspecs_eq by trivial.
-  apply (@Canonical_semax_func _ _ _ _ _ _ _ _ Comp); cbv; reflexivity.
-  destruct MAIN as [post [MainG MainExp]]. inv MainExp. rewrite MainG; eexists; reflexivity.
-Qed.
-
-(* Print Assumptions prog_correct. *)
