progs/VSUpile/simple_verif_onepile.v
@@ -5,13 +5,13 @@ Require Import simple_spec_stdlib.
 Require Import simple_spec_pile.
 Require Import simple_spec_onepile.
 
-  Definition onepile_imported_specs:funspecs := 
+Definition onepile_imported_specs:funspecs := 
      [ Pile_new_spec; Pile_add_spec; Pile_count_spec].
 
-  Definition onepile_internal_specs: funspecs := OnepileASI.
+Definition onepile_internal_specs: funspecs := OnepileASI.
 
-  Definition OnepileVprog: varspecs. mk_varspecs prog. Defined.
-  Definition OnepileGprog: funspecs := onepile_imported_specs ++ onepile_internal_specs.
+Definition OnepileVprog: varspecs. mk_varspecs prog. Defined.
+Definition OnepileGprog: funspecs := onepile_imported_specs ++ onepile_internal_specs.
 
 Lemma body_Onepile_init: semax_body OnepileVprog OnepileGprog f_Onepile_init Onepile_init_spec.
 Proof.
@@ -50,48 +50,17 @@ Exists p.
 entailer!.
 Qed.
 
+Lemma onepile_Init: VSU_initializer prog (onepile None).
+Proof. InitGPred_tac. normalize. apply derives_refl. Qed.
 
-Lemma make_onepile: forall gv,
-  data_at_ Ews (tptr (Tstruct onepile._pile noattr)) (gv onepile._the_pile)
-   |-- onepile None gv.
-Proof.
-intros. cancel.
-Qed.
 
-  Lemma onepile_Init_aux gv: headptr (gv _the_pile) ->
-    globvar2pred gv (_the_pile, v_the_pile)
-    |-- data_at_ Ews (tptr (Tstruct _pile noattr)) (gv _the_pile).
-  Proof. intros.
-    unfold globvar2pred. simpl.
-         rewrite sepcon_emp.
-    destruct H as [b Hb]; rewrite Hb in *.
-    eapply derives_trans. 
-    + apply mapsto_zeros_memory_block. apply writable_readable. apply writable_Ews.
-    + rewrite <- memory_block_data_at_; simpl; trivial.
-      apply headptr_field_compatible; trivial. exists b; trivial. cbv; trivial. simpl; rep_lia.
-      econstructor. reflexivity. apply Z.divide_0_r.
-  Qed.
-
-(*
-  Lemma onepile_Init_aux2 gv: headptr (gv _the_pile) ->
-    globvar2pred gv (_the_pile, v_the_pile)
-    |--  onepile None gv.
-  Proof. intros. sep_apply onepile_Init_aux. apply make_onepile; trivial. Qed.
-*)
-
-  Lemma onepile_Init gv: globals_ok gv -> InitGPred (Vardefs prog) gv |-- onepile None gv.
-  Proof. InitGPred_tac. normalize. apply derives_refl. Qed.
-
-  Definition OnepileComponent: @Component NullExtension.Espec OnepileVprog _ 
-      nil onepile_imported_specs prog OnepileASI (onepile None) onepile_internal_specs.
+Definition OnepileVSU: @VSU NullExtension.Espec
+      nil onepile_imported_specs ltac:(QPprog prog) OnepileASI (onepile None).
   Proof.
-    mkComponent. 
+    mkVSU prog onepile_internal_specs. 
+    + solve_SF_internal body_Onepile_count.
     + solve_SF_internal body_Onepile_init.
     + solve_SF_internal body_Onepile_add.
-    + solve_SF_internal body_Onepile_count.
     + apply onepile_Init.
   Qed.
 
-Definition OnepileVSU: @VSU NullExtension.Espec OnepileVprog _ 
-      nil onepile_imported_specs prog OnepileASI (onepile None).
-  Proof. eexists; apply OnepileComponent. Qed.
